- Propagated changes to the modified Coq file - Propagated changes to extractable file - Fixed the following things:   * Now the extractable relation takes the selection as a parameter   * However, it is unable to "guess" the selection parameter to pass downstream, therefore I introduced a coinductive datatype selectstar, which describes the full (infinite) downstream path if needed (it is only needed for trees of forks). This makes this change fairly complex in theory - Performed full extraction, but it appears the full extractable semantics is too big for the extraction plugin (stack overflows and broken pipes all over). Therefore I have done it piece-by-piece (see extractedPieces.txt) which I will hand reassemble.

mconbase2.v
@@ -31,19 +31,24 @@ Inductive typexpr : Set :=
 Inductive constant : Set := 
  | CONST_ret : constant
  | CONST_fork : constant
- | CONST_unit : constant.
+ | CONST_unit : constant
+ | CONST_stop : constant.
 
 Inductive list_typvar : Set := 
  | Nil_list_typvar : list_typvar
  | Cons_list_typvar (_:typvar) (_:list_typvar).
 
-Inductive expr : Set := 
+Inductive livemodes : Set := 
+ | LM_comp : livemodes
+ | LM_expr (expr5:expr)
+with expr : Set := 
  | E_ident (value_name5:value_name)
  | E_constant (constant5:constant)
  | E_apply (expr5:expr) (expr':expr)
  | E_bind (expr5:expr) (expr':expr)
  | E_function (value_name5:value_name) (typexpr5:typexpr) (expr5:expr)
- | E_live_expr (expr5:expr)
+ | E_fix (e:expr)
+ | E_live_expr (lm:livemodes)
  | E_pair (e:expr) (e':expr)
  | E_taggingleft (e:expr)
  | E_taggingright (e:expr)
@@ -51,6 +56,10 @@ Inductive expr : Set :=
 
 Inductive typscheme : Set := 
  | TS_ts (_:list_typvar) (typexpr5:typexpr).
+
+Inductive select : Set := 
+ | S_First : select
+ | S_Second : select.
 
 Inductive G : Set := 
  | G_em : G
@@ -100,11 +109,12 @@ Fixpoint is_value_of_expr (e_5:expr) : Prop :=
   match e_5 with
   | (E_ident value_name5) => False
   | (E_constant constant5) => (True)
-(* Manual addition *)
-  | (E_apply expr5 expr') => match expr5 with | E_constant (CONST_fork) => ((is_value_of_expr expr')) | _ => False end
+(* Manual change *)
+  | (E_apply expr5 expr') => match expr5 with | E_constant (CONST_fork) => is_value_of_expr (expr') | _ => False end
   | (E_bind expr5 expr') => False
   | (E_function value_name5 typexpr5 expr5) => (True)
-  | (E_live_expr expr5) => (True)
+  | (E_fix e) => ((is_value_of_expr e))
+  | (E_live_expr lm) => (True)
   | (E_pair e e') => ((is_value_of_expr e) /\ (is_value_of_expr e'))
   | (E_taggingleft e) => ((is_value_of_expr e))
   | (E_taggingright e) => ((is_value_of_expr e))
@@ -150,20 +160,6 @@ Definition tsubst_typscheme (sub:list (typvar*typexpr)) (ts5:typscheme) : typsch
   | (TS_ts typvar_list typexpr5) => TS_ts typvar_list (tsubst_typexpr (list_minus2 eq_typvar sub (unmake_list_typvar typvar_list)) typexpr5)
 end.
 
-Fixpoint subst_expr (e_5:expr) (x_5:value_name) (e__6:expr) {struct e__6} : expr :=
-  match e__6 with
-  | (E_ident value_name5) => (if eq_value_name value_name5 x_5 then e_5 else (E_ident value_name5))
-  | (E_constant constant5) => E_constant constant5
-  | (E_apply expr5 expr') => E_apply (subst_expr e_5 x_5 expr5) (subst_expr e_5 x_5 expr')
-  | (E_bind expr5 expr') => E_bind (subst_expr e_5 x_5 expr5) (subst_expr e_5 x_5 expr')
-  | (E_function value_name5 typexpr5 expr5) => E_function value_name5 typexpr5 (if list_mem eq_value_name x_5 (cons value_name5 nil) then expr5 else (subst_expr e_5 x_5 expr5))
-  | (E_live_expr expr5) => E_live_expr (subst_expr e_5 x_5 expr5)
-  | (E_pair e e') => E_pair (subst_expr e_5 x_5 e) (subst_expr e_5 x_5 e')
-  | (E_taggingleft e) => E_taggingleft (subst_expr e_5 x_5 e)
-  | (E_taggingright e) => E_taggingright (subst_expr e_5 x_5 e)
-  | (E_case e1 x1 e2 x2 e3) => E_case (subst_expr e_5 x_5 e1) x1 (subst_expr e_5 x_5 e2) x2 (subst_expr e_5 x_5 e3)
-end.
-
 Fixpoint tsubst_expr (sub:list (typvar*typexpr)) (e_5:expr) {struct e_5} : expr :=
   match e_5 with
   | (E_ident value_name5) => E_ident value_name5
@@ -171,17 +167,43 @@ Fixpoint tsubst_expr (sub:list (typvar*typexpr)) (e_5:expr) {struct e_5} : expr 
   | (E_apply expr5 expr') => E_apply (tsubst_expr sub expr5) (tsubst_expr sub expr')
   | (E_bind expr5 expr') => E_bind (tsubst_expr sub expr5) (tsubst_expr sub expr')
   | (E_function value_name5 typexpr5 expr5) => E_function value_name5 (tsubst_typexpr sub typexpr5) (tsubst_expr sub expr5)
-  | (E_live_expr expr5) => E_live_expr (tsubst_expr sub expr5)
+  | (E_fix e) => E_fix (tsubst_expr sub e)
+  | (E_live_expr lm) => E_live_expr (tsubst_livemodes sub lm)
   | (E_pair e e') => E_pair (tsubst_expr sub e) (tsubst_expr sub e')
   | (E_taggingleft e) => E_taggingleft (tsubst_expr sub e)
   | (E_taggingright e) => E_taggingright (tsubst_expr sub e)
   | (E_case e1 x1 e2 x2 e3) => E_case (tsubst_expr sub e1) x1 (tsubst_expr sub e2) x2 (tsubst_expr sub e3)
+end
+with tsubst_livemodes (sub:list (typvar*typexpr)) (lm5:livemodes) {struct lm5} : livemodes :=
+  match lm5 with
+  | LM_comp => LM_comp 
+  | (LM_expr expr5) => LM_expr (tsubst_expr sub expr5)
 end.
 
 Fixpoint tsubst_G (sub:list (typvar*typexpr)) (G_6:G) {struct G_6} : G :=
   match G_6 with
   | G_em => G_em 
   | (G_vn G5 value_name5 typscheme5) => G_vn (tsubst_G sub G5) value_name5 (tsubst_typscheme sub typscheme5)
+end.
+
+Fixpoint subst_expr (e_5:expr) (x_5:value_name) (e__6:expr) {struct e__6} : expr :=
+  match e__6 with
+  | (E_ident value_name5) => (if eq_value_name value_name5 x_5 then e_5 else (E_ident value_name5))
+  | (E_constant constant5) => E_constant constant5
+  | (E_apply expr5 expr') => E_apply (subst_expr e_5 x_5 expr5) (subst_expr e_5 x_5 expr')
+  | (E_bind expr5 expr') => E_bind (subst_expr e_5 x_5 expr5) (subst_expr e_5 x_5 expr')
+  | (E_function value_name5 typexpr5 expr5) => E_function value_name5 typexpr5 (if list_mem eq_value_name x_5 (cons value_name5 nil) then expr5 else (subst_expr e_5 x_5 expr5))
+  | (E_fix e) => E_fix (subst_expr e_5 x_5 e)
+  | (E_live_expr lm) => E_live_expr (subst_livemodes e_5 x_5 lm)
+  | (E_pair e e') => E_pair (subst_expr e_5 x_5 e) (subst_expr e_5 x_5 e')
+  | (E_taggingleft e) => E_taggingleft (subst_expr e_5 x_5 e)
+  | (E_taggingright e) => E_taggingright (subst_expr e_5 x_5 e)
+  | (E_case e1 x1 e2 x2 e3) => E_case (subst_expr e_5 x_5 e1) x1 (subst_expr e_5 x_5 e2) x2 (subst_expr e_5 x_5 e3)
+end
+with subst_livemodes (e5:expr) (x5:value_name) (lm5:livemodes) {struct lm5} : livemodes :=
+  match lm5 with
+  | LM_comp => LM_comp 
+  | (LM_expr expr5) => LM_expr (subst_expr e5 x5 expr5)
 end.
 
 (** library functions *)
@@ -216,11 +238,17 @@ Fixpoint ftv_expr (e_5:expr) : list typvar :=
   | (E_apply expr5 expr') => (app (ftv_expr expr5) (ftv_expr expr'))
   | (E_bind expr5 expr') => (app (ftv_expr expr5) (ftv_expr expr'))
   | (E_function value_name5 typexpr5 expr5) => (app (ftv_typexpr typexpr5) (ftv_expr expr5))
-  | (E_live_expr expr5) => ((ftv_expr expr5))
+  | (E_fix e) => ((ftv_expr e))
+  | (E_live_expr lm) => ((ftv_livemodes lm))
   | (E_pair e e') => (app (ftv_expr e) (ftv_expr e'))
   | (E_taggingleft e) => ((ftv_expr e))
   | (E_taggingright e) => ((ftv_expr e))
   | (E_case e1 x1 e2 x2 e3) => (app (ftv_expr e1) (app (ftv_expr e2) (ftv_expr e3)))
+end
+with ftv_livemodes (lm5:livemodes) : list typvar :=
+  match lm5 with
+  | LM_comp => nil
+  | (LM_expr expr5) => ((ftv_expr expr5))
 end.
 
 Fixpoint ftv_G (G_6:G) : list typvar :=
@@ -254,6 +282,8 @@ with G_constant : G -> constant -> typexpr -> Prop :=    (* defn G_constant *)
      G_constant G5 CONST_fork (TE_arrow  (TE_concurrent t1)   (TE_arrow  (TE_concurrent t2)   (TE_concurrent  (TE_sum  (TE_sum  (TE_prod t1 t2)   (TE_prod t1  (TE_concurrent t2) ) )   (TE_prod  (TE_concurrent t1)  t2) ) ) ) )
  | constant_unit : forall (G5:G),
      G_constant G5 CONST_unit (TE_constants TC_unit)
+ | constant_stop : forall (G5:G) (t:typexpr),
+     G_constant G5 CONST_stop t
 with Get : G -> expr -> typexpr -> Prop :=    (* defn Get *)
  | Get_value_name : forall (G5:G) (x:value_name) (t:typexpr) (typscheme5:typscheme),
      VTSin x typscheme5 G5 ->
@@ -274,9 +304,14 @@ with Get : G -> expr -> typexpr -> Prop :=    (* defn Get *)
  | Get_lambda : forall (G5:G) (x1:value_name) (t1:typexpr) (e:expr) (t:typexpr),
      Get (G_vn G5 x1 (TS_ts Nil_list_typvar t1)) e t ->
      Get G5 (E_function x1 t1 e) (TE_arrow t1 t)
- | Get_live : forall (G5:G) (e:expr) (t:typexpr),
+ | Get_live_exp : forall (G5:G) (e:expr) (t:typexpr),
      Get G5 e t ->
-     Get G5 (E_live_expr e) (TE_concurrent t)
+     Get G5 (E_live_expr (LM_expr e)) (TE_concurrent t)
+ | Get_live_comp : forall (G5:G),
+     Get G5 (E_live_expr LM_comp) (TE_concurrent (TE_constants TC_unit))
+ | Get_fix : forall (G5:G) (e:expr) (t:typexpr),
+     Get G5 e (TE_arrow t t) ->
+     Get G5 (E_fix e) t
  | Get_bind : forall (G5:G) (e e':expr) (t' t:typexpr),
      Get G5 e (TE_concurrent t) ->
      Get G5 e' (TE_arrow t (TE_concurrent t')) ->
@@ -299,68 +334,83 @@ with Get : G -> expr -> typexpr -> Prop :=    (* defn Get *)
 (** definitions *)
 
 (* defns Jop *)
-Inductive JO_red : expr -> expr -> Prop :=    (* defn red *)
- | JO_red_app : forall (x:value_name) (t:typexpr) (e v:expr),
+Inductive JO_red : expr -> select -> expr -> Prop :=    (* defn red *)
+ | JO_red_app : forall (x:value_name) (t:typexpr) (e:expr) (s:select) (v:expr),
      is_value_of_expr v ->
-     JO_red (E_apply  (E_function x t e)  v)  (subst_expr  v   x   e ) 
- | JO_red_forkmove1 : forall (e e' e'':expr),
+     JO_red (E_apply  (E_function x t e)  v) s  (subst_expr  v   x   e ) 
+ | JO_red_forkmove1 : forall (e e' e'':expr) (s:select),
      ~ ( is_value_of_expr ( e' ) )  ->
-     JO_red e e'' ->
-     JO_red (E_apply  (E_apply (E_constant CONST_fork)  (E_live_expr e) )   (E_live_expr e') ) (E_apply  (E_apply (E_constant CONST_fork)  (E_live_expr e'') )   (E_live_expr e') )
- | JO_red_forkmove2 : forall (e e' e'':expr),
+     JO_red e s e'' ->
+     JO_red (E_apply  (E_apply (E_constant CONST_fork)  (E_live_expr (LM_expr e)) )   (E_live_expr (LM_expr e')) ) S_First (E_apply  (E_apply (E_constant CONST_fork)  (E_live_expr (LM_expr e'')) )   (E_live_expr (LM_expr e')) )
+ | JO_red_forkmove2 : forall (e e' e'':expr) (s:select),
      ~ ( is_value_of_expr ( e ) )  ->
-     JO_red e' e'' ->
-     JO_red (E_apply  (E_apply (E_constant CONST_fork)  (E_live_expr e) )   (E_live_expr e') ) (E_apply  (E_apply (E_constant CONST_fork)  (E_live_expr e) )   (E_live_expr e'') )
- | JO_red_forkdeath1 : forall (v e':expr),
+     JO_red e' s e'' ->
+     JO_red (E_apply  (E_apply (E_constant CONST_fork)  (E_live_expr (LM_expr e)) )   (E_live_expr (LM_expr e')) ) S_Second (E_apply  (E_apply (E_constant CONST_fork)  (E_live_expr (LM_expr e)) )   (E_live_expr (LM_expr e'')) )
+ | JO_red_forkdeath1 : forall (v e:expr) (s:select),
      is_value_of_expr v ->
-     JO_red (E_apply  (E_apply (E_constant CONST_fork)  (E_live_expr v) )   (E_live_expr e') ) (E_live_expr (E_pair v  (E_live_expr e') ))
- | JO_red_forkdeath2 : forall (e v:expr),
-     is_value_of_expr v ->
-     JO_red (E_apply  (E_apply (E_constant CONST_fork)  (E_live_expr e) )   (E_live_expr v) ) (E_live_expr (E_pair  (E_live_expr e)  v))
- | JO_red_forkdeath12 : forall (v v':expr),
+     JO_red (E_apply  (E_apply (E_constant CONST_fork)  (E_live_expr (LM_expr v)) )   (E_live_expr (LM_expr e)) ) s (E_live_expr (LM_expr  (E_taggingleft  (E_taggingright  (E_pair v  (E_live_expr (LM_expr e)) ) ) ) ))
+ | JO_red_forkdeath2 : forall (e v':expr) (s:select),
+     is_value_of_expr v' ->
+     JO_red (E_apply  (E_apply (E_constant CONST_fork)  (E_live_expr (LM_expr e)) )   (E_live_expr (LM_expr v')) ) s (E_live_expr (LM_expr  (E_taggingright  (E_pair  (E_live_expr (LM_expr e))  v') ) ))
+ | JO_red_forkdeath12 : forall (v v':expr) (s:select),
      is_value_of_expr v ->
      is_value_of_expr v' ->
-     JO_red (E_apply  (E_apply (E_constant CONST_fork)  (E_live_expr v) )   (E_live_expr v') ) (E_live_expr (E_pair v v'))
- | JO_red_ret : forall (v:expr),
+     JO_red (E_apply  (E_apply (E_constant CONST_fork)  (E_live_expr (LM_expr v)) )   (E_live_expr (LM_expr v')) ) s (E_live_expr (LM_expr  (E_taggingleft  (E_taggingleft  (E_pair v v') ) ) ))
+ | JO_red_forkdocomp1 : forall (e:expr) (s:select),
+     JO_red (E_apply  (E_apply (E_constant CONST_fork)  (E_live_expr LM_comp) )   (E_live_expr (LM_expr e)) ) s (E_live_expr (LM_expr  (E_taggingleft  (E_taggingright  (E_pair (E_constant CONST_unit)  (E_live_expr (LM_expr e)) ) ) ) ))
+ | JO_red_forkdocomp2 : forall (e:expr) (s:select),
+     JO_red (E_apply  (E_apply (E_constant CONST_fork)  (E_live_expr (LM_expr e)) )   (E_live_expr LM_comp) ) s (E_live_expr (LM_expr  (E_taggingright  (E_pair  (E_live_expr (LM_expr e))  (E_constant CONST_unit)) ) ))
+ | JO_red_forkdocomp12 : forall (s:select),
+     JO_red (E_apply  (E_apply (E_constant CONST_fork)  (E_live_expr LM_comp) )   (E_live_expr LM_comp) ) s (E_live_expr (LM_expr  (E_taggingleft  (E_taggingleft  (E_pair (E_constant CONST_unit) (E_constant CONST_unit)) ) ) ))
+ | JO_red_ret : forall (v:expr) (s:select),
      is_value_of_expr v ->
-     JO_red (E_apply (E_constant CONST_ret) v) (E_live_expr v)
- | JO_red_evalbind : forall (e e'' e':expr),
-     JO_red e e' ->
-     JO_red (E_bind e e'') (E_bind e' e'')
- | JO_red_movebind : forall (e e'' e':expr),
-     JO_red e e' ->
-     JO_red (E_bind  (E_live_expr e)  e'') (E_bind  (E_live_expr e')  e'')
- | JO_red_dobind : forall (v e:expr),
+     JO_red (E_apply (E_constant CONST_ret) v) s  (E_live_expr (LM_expr v)) 
+ | JO_red_evalbind : forall (e e'':expr) (s:select) (e':expr),
+     JO_red e s e' ->
+     JO_red (E_bind e e'') s (E_bind e' e'')
+ | JO_red_movebind : forall (e e'':expr) (s:select) (e':expr),
+     JO_red e s e' ->
+     JO_red (E_bind  (E_live_expr (LM_expr e))  e'') s (E_bind  (E_live_expr (LM_expr e'))  e'')
+ | JO_red_compbind : forall (e:expr) (s:select) (e':expr),
+     JO_red (E_bind  (E_live_expr LM_comp)  e) s (E_apply e' (E_constant CONST_unit))
+ | JO_red_dobind : forall (v e:expr) (s:select),
      is_value_of_expr v ->
-     JO_red (E_bind  (E_live_expr v)  e) (E_apply e v)
- | JO_red_context_app1 : forall (e e' e'':expr),
-     JO_red e' e'' ->
-     JO_red (E_apply e e') (E_apply e e'')
- | JO_red_context_app2 : forall (e v e':expr),
+     JO_red (E_bind  (E_live_expr (LM_expr v))  e) s (E_apply e v)
+ | JO_red_context_app1 : forall (e e':expr) (s:select) (e'':expr),
+     JO_red e' s e'' ->
+     JO_red (E_apply e e') s (E_apply e e'')
+ | JO_red_context_app2 : forall (e v:expr) (s:select) (e':expr),
      is_value_of_expr v ->
-     JO_red e e' ->
-     JO_red (E_apply e v) (E_apply e' v)
- | JO_red_pair_1 : forall (e e'' e':expr),
-     JO_red e e' ->
-     JO_red (E_pair e e'') (E_pair e' e'')
- | JO_red_pair_2 : forall (v e e':expr),
+     JO_red e s e' ->
+     JO_red (E_apply e v) s (E_apply e' v)
+ | JO_red_fix_move : forall (e:expr) (s:select) (e':expr),
+     JO_red e s e' ->
+     JO_red  (E_fix e)  s  (E_fix e') 
+ | JO_red_fix_app : forall (v v':expr) (s:select),
      is_value_of_expr v ->
-     JO_red e e' ->
-     JO_red (E_pair v e) (E_pair v e')
- | JO_red_evalinl : forall (e e':expr),
-     JO_red e e' ->
-     JO_red (E_taggingleft e) (E_taggingleft e')
- | JO_red_evalinr : forall (e e':expr),
-     JO_red e e' ->
-     JO_red (E_taggingright e) (E_taggingright e')
- | JO_red_evalcaseinl : forall (x:value_name) (e:expr) (x':value_name) (e' v:expr),
+     is_value_of_expr v' ->
+     JO_red (E_apply  (E_fix v)  v') s (E_apply  (E_fix v)   (E_apply v v') )
+ | JO_red_pair_1 : forall (e e'':expr) (s:select) (e':expr),
+     JO_red e s e' ->
+     JO_red (E_pair e e'') s (E_pair e' e'')
+ | JO_red_pair_2 : forall (v e:expr) (s:select) (e':expr),
      is_value_of_expr v ->
-     JO_red (E_case  (E_taggingleft v)  x e x' e')  (subst_expr  v   x   e ) 
- | JO_red_evalcaseinr : forall (x:value_name) (e:expr) (x':value_name) (e' v:expr),
+     JO_red e s e' ->
+     JO_red (E_pair v e) s (E_pair v e')
+ | JO_red_evalinl : forall (e:expr) (s:select) (e':expr),
+     JO_red e s e' ->
+     JO_red (E_taggingleft e) s (E_taggingleft e')
+ | JO_red_evalinr : forall (e:expr) (s:select) (e':expr),
+     JO_red e s e' ->
+     JO_red (E_taggingright e) s (E_taggingright e')
+ | JO_red_evalcaseinl : forall (x:value_name) (e:expr) (x':value_name) (e':expr) (s:select) (v:expr),
      is_value_of_expr v ->
-     JO_red (E_case  (E_taggingright v)  x e x' e')  (subst_expr  v   x'   e' ) 
- | JO_red_evalcase : forall (e:expr) (x:value_name) (e'':expr) (x':value_name) (e''' e':expr),
-     JO_red e e' ->
-     JO_red (E_case e x e'' x' e''') (E_case e' x e'' x' e''').
+     JO_red (E_case  (E_taggingleft v)  x e x' e') s  (subst_expr  v   x   e ) 
+ | JO_red_evalcaseinr : forall (x:value_name) (e:expr) (x':value_name) (e':expr) (s:select) (v:expr),
+     is_value_of_expr v ->
+     JO_red (E_case  (E_taggingright v)  x e x' e') s  (subst_expr  v   x'   e' ) 
+ | JO_red_evalcase : forall (e:expr) (x:value_name) (e'':expr) (x':value_name) (e''':expr) (s:select) (e':expr),
+     JO_red e s e' ->
+     JO_red (E_case e x e'' x' e''') s (E_case e' x e'' x' e''').
 
 
