mconextract.v
@@ -10,14 +10,6 @@ Require Import Classical_Prop.
 
 Load mconbase2.
 
-Inductive selectSet : Set := 
- | First : selectSet
- | Second : selectSet
- | Both : selectSet.
-
-Axiom select : selectSet.
-
-Extract Constant select => "(selectBranch)".
 
 
 (* Extractable version of is_value_of_expr *)
@@ -29,6 +21,7 @@ Fixpoint xis_value_of_expr (e_5:expr) : bool :=
   | (E_apply expr5 expr') => false
   | (E_bind expr5 expr') => false
   | (E_function value_name5 typexpr5 expr5) => true
+  | (E_fix e) => ((xis_value_of_expr e))
   | (E_live_expr expr5) => true
   | (E_pair e e') => (if (xis_value_of_expr e) then (xis_value_of_expr e') else false)
   | (E_taggingleft e) => ((xis_value_of_expr e))
@@ -36,1137 +29,155 @@ Fixpoint xis_value_of_expr (e_5:expr) : bool :=
   | (E_case e1 x1 e2 x2 e3) => false
 end.
 
+(*
+Fixpoint xis_forkvalue (e : expr) : bool :=
+  match e with
+  | (E_ident value_name5) => false
+  | (E_constant constant5) => match constant5 with | CONST_fork => false | CONST_ret => true | CONST_unit => false | CONST_stop => true end
+  | (E_apply (E_constant (CONST_fork)) e) => ((xis_value_of_expr e))
+  | (E_apply expr5 expr') => false
+  | (E_bind expr5 expr') => false
+  | (E_function value_name5 typexpr5 expr5) => false
+  | (E_fix e) => (xis_value_of_expr e)
+  | (E_live_expr lm) => match lm with | LM_comp => false | LM_expr e' => (xis_value_of_expr e') end
+  | (E_pair e e') => false
+  | (E_taggingleft e) => false
+  | (E_taggingright e) => false
+  | (E_case e1 x1 e2 x2 e3) => false
+end. *)
+
 (* Proof that is_value_of_expr and xis_value_of_expr are equivalent *)
 
-Lemma l_val : forall (e:expr), (eq (xis_value_of_expr e) true) <-> (is_value_of_expr e).
-Proof.
- intros.
- split.
- (* xis -> is*)
-  intros.
-  induction e.
-  (* ident *)
-   simpl in H.
-   apply diff_true_false.
-   symmetry.
-   trivial.
-  (* constant *)
-   simpl.
-   trivial.
-  (* apply *)
-   induction e1.
-   inversion H.
-   case_eq constant5.
-   intros.
-   rewrite -> H0 in H.
-   inversion H.
-   intros.
-   rewrite -> H0 in H.
-   rewrite -> H0 in IHe1.
-   simpl.
-   apply IHe2.
-   inversion H.
-   reflexivity.
-   intros.
-   rewrite -> H0 in H.
-   inversion H.
-   inversion H.
-   inversion H.
-   simpl.
-   simpl in H.
-   congruence.
-   inversion H.
-   inversion H.
-   inversion H.
-   inversion H.
-   inversion H.
-  (* bind *) 
-   simpl.
-   trivial.
-   simpl in H.
-   apply diff_true_false.
-   symmetry.
-   trivial.
-  (* function *) 
-   simpl; trivial.
-  (* live *)
-   simpl; trivial.
-  (* pair *)
-   simpl in H.
-   simpl.
-   split.
-   destruct (xis_value_of_expr e1).
-   auto.
-   auto.
-   destruct (xis_value_of_expr e2).
-   auto.
-   destruct (xis_value_of_expr e1).
-   auto.
-   auto.
-  (* tagging left *)
-   simpl.
-   auto.
-  (* tagging right *) 
-   simpl.
-   auto.
-  (* case *) 
-   simpl in H.
-   simpl.
-   apply diff_true_false.
-   symmetry.
-   trivial.
- (* is -> xis *)
-  intros.
-  induction e.
-  (* ident *) 
-   simpl in H.
-   contradiction.
-  (* constant *)
-   simpl; trivial.
-  (* apply *)
-   induction e1.
-   simpl in H.
-   elim H.
-   simpl in H.
-   case_eq constant5.
-   intros.
-   rewrite -> H0 in H.
-   elim H.
-   intros.
-   rewrite -> H0 in H.
-   simpl.
-   apply IHe2.
-   trivial.
-   intros.
-   rewrite -> H0 in H.
-   auto.
-   simpl in H.
-   simpl in H.
-   elim H.
-   simpl in H.
-   elim H.
-   simpl in H.
-   elim H.
-   simpl in H.
-   elim H.
-   simpl in H.
-   elim H.
-   simpl in H.
-   elim H.
-   simpl in H.
-   elim H.
-   simpl in H; contradiction.
-  (* bind *)
-   simpl in H; contradiction.
-  (* function *)
-   simpl; trivial.
-  (* live *)
-   simpl; trivial.
-  (* pair *)
-   simpl in H.
-   decompose [and] H. 
-   simpl in IHe1.
-   simpl.
-   rewrite IHe1.
-   auto.
-   auto.
-  (* tagging left *)
-   simpl; simpl in H; auto.
-  (* tagging right *)
-   simpl; simpl in H; auto.
-  (* case *)
-   simpl; contradiction.
-Qed.
+CoInductive selectstar : Set := Seq : select -> selectstar -> selectstar.
 
-Hint Resolve eq_value_name : ott_coq_equality.
-(*
-Lemma eq_typscheme: forall (x y : typscheme), {x = y} + {x <> y}.
-Proof.
-decide equality. decide equality. apply eq_typvar. decide equality. apply eq_typvar.
-Defined.
-Hint Resolve eq_typscheme : ott_coq_equality.
-
-(* Extractable VTSin *)
-
-Fixpoint XVTSin (v : value_name) (ts : typscheme)  (G5 : G) : bool := 
- match G5 with 
- | G_em => false 
- | G_vn (G6 ) (v' ) (ts' ) => if (eq_value_name v v') then ( if (eq_typscheme ts ts') then true else false) else XVTSin v ts G6
-end.
-
-(* Proof that the extractable VTSin is the same as the original *)
-
-Lemma xvtsin_eq_vtsin : forall (v : value_name) (ts : typscheme)  (G5 : G), XVTSin v ts G5 = true <-> VTSin v ts G5.
-Proof.
- intros.
- split.
- intros.
- induction G5.
- simpl in H.
- symmetry in H.
- apply diff_true_false in H.
- contradiction.
- destruct (eq_value_name v value_name5).
- rewrite <- e.
- destruct (eq_typscheme ts typscheme5).
- rewrite <- e0.
- apply VTSin_vn1.
- apply VTSin_vn2.
- apply IHG5.
- rewrite <- e in H.
- simpl in H.
- destruct (eq_value_name v v).
- destruct (eq_typscheme ts typscheme5).
- contradiction.
- symmetry in H.
- apply diff_true_false in H.
- contradiction.
- trivial.
- rewrite <- e in H.
- simpl in H.
- destruct (eq_value_name v v).
- destruct (eq_typscheme ts typscheme5).
- contradiction.
- symmetry in H.
- apply diff_true_false in H.
- contradiction.
- trivial.
- simpl in H.
- destruct (eq_value_name v value_name5).
- contradiction.
- apply VTSin_vn2.
- apply IHG5.
- trivial.
- trivial.
- intros.
- induction G5.
- inversion H.
- simpl.
- destruct (eq_value_name v value_name5).
- rewrite <- e in H.
- destruct (eq_typscheme ts typscheme5).
- trivial.
- inversion H.
- rewrite -> H4 in n.
- cut (typscheme5 = typscheme5).
- intros.
- contradiction.
- auto.
- cut (v = v).
- intros.
- contradiction.
- auto.
- inversion H.
- contradiction.
- apply IHG5.
- trivial.
-Qed.
-
-Fixpoint GetTS (v : value_name)  (G5 : G)  : option typscheme :=
-match G5 with 
- | G_em => None 
- | G_vn (G6 ) (v' ) (ts' ) => if (eq_value_name v v') then ( Some ts') else GetTS v G6
-end.
-
-Lemma eq_typexpr: forall (x y : typexpr), {x = y} + {x <> y}.
-Proof.
-decide equality. apply eq_typvar. 
-Defined.
-Hint Resolve eq_typexpr : ott_coq_equality.
-
-Fixpoint newTV0 (l : list_typvar) (s : nat) : typvar :=
- match l with 
- | Nil_list_typvar => TV_ident(s)
- | Cons_list_typvar (TV_ident (n)) l' => newTV0 l' (s+n+1)
-end.
-
-Fixpoint newTV (l : list_typvar) : typvar := 
- let newTV0 (lt : list_typvar) (s : nat) : typvar :=
- match l with 
- | Nil_list_typvar => TV_ident(s)
- | Cons_list_typvar (TV_ident (n)) lt' => newTV0 lt' (s+n+1)
- end in
- newTV0 l 0.
-
-Fixpoint generalise (G5 : G) (T : typexpr) : typscheme := (TS_ts (remove_duplicates (make_list_typvar (list_minus eq_typvar (ftv_typexpr T) (ftv_G G5)))) T).
-
-Fixpoint occurs (v : typvar) (e : typexpr) : bool :=
- match e with
- | TE_var (typvar5 ) => if eq_typvar v typvar5 then true else false
- | TE_arrow (typexpr5) (typexpr') => orb (occurs v typexpr5) (occurs v typexpr')
- | TE_prod (typexpr5) (typexpr') => orb (occurs v typexpr5) (occurs v typexpr')
- | TE_concurrent (typexpr5) => occurs v typexpr5
- | TE_sum (typexpr5) (typexpr') => orb (occurs v typexpr5) (occurs v typexpr')
-end.
-
-Fixpoint mgu (e1 : typexpr) (e2 : typexpr)  : option (list (typvar*typexpr))  :=
- match e1 with 
- | TE_var (typvar5 ) => if (occurs typvar5 e2) 
-                         then match e2 with 
-                              | TE_var (typvar6 ) => Some (cons (pair typvar5 e2) nil)
-                              | _ => None
-                              end
-                         else Some (cons (pair typvar5 e2) nil)
- | TE_arrow (typexpr5) (typexpr') => 
-    match e2 with 
-    | TE_var (typvar5 ) => if (occurs typvar5 e1) then None else Some (cons (pair typvar5 e1) nil)
-    | TE_arrow (typexpr6) (typexpr'') => match mgu typexpr5 typexpr6 with
-                                         | None => None
-                                         | Some l => match mgu (tsubst_typexpr l typexpr') typexpr'' with
-                                                     | None => None
-                                                     | Some l' => Some (app l l') 
-                                                     end
-                                         end
-    | _ => None
-    end
- | TE_prod (typexpr5) (typexpr') => 
-     match e2 with 
-    | TE_var (typvar5 ) => if (occurs typvar5 e1) then None else Some (cons (pair typvar5 e1) nil)
-    | TE_prod (typexpr6) (typexpr'') => match mgu typexpr5 typexpr6 with
-                                         | None => None
-                                         | Some l => match mgu (tsubst_typexpr l typexpr') typexpr'' with
-                                                     | None => None
-                                                     | Some l' => Some (app l l')
-                                                     end
-                                         end
-    | _ => None
-    end
- | TE_concurrent (typexpr5) => 
-    match e2 with 
-    | TE_var (typvar5 ) => if (occurs typvar5 e1) then None else Some (cons (pair typvar5 e1) nil)
-    | TE_concurrent (typexpr6) => mgu typexpr5 typexpr6
-    | _ => None
-    end
- | TE_sum (typexpr5) (typexpr') => 
-    match e2 with 
-    | TE_var (typvar5 ) => if (occurs typvar5 e1) then None else Some (cons (pair typvar5 e1) nil)
-    | TE_sum (typexpr6) (typexpr'') => match mgu typexpr5 typexpr6 with
-                                         | None => None
-                                         | Some l => match mgu (tsubst_typexpr l typexpr') typexpr'' with
-                                                     | None => None
-                                                     | Some l' => Some (app l l')
-                                                     end
-                                         end
-    | _ => None
-    end
-end.
-
-Lemma empty_sub : forall (tv : typvar) (texp0 texp : typexpr), (occurs tv texp = false) ->  (tsubst_typexpr ((pair tv texp0)::nil) texp) = texp.
-Proof. 
- intros.
- induction texp.
- simpl.
- simpl in H.
- destruct (eq_typvar tv typvar5).
- congruence.
- reflexivity.
- simpl in H.
- case_eq (occurs tv texp1).
- intros.
- rewrite -> H0 in H.
- simpl in H.
- congruence.
- intros. case_eq (occurs tv texp2). intros. 
- rewrite -> H1 in H. rewrite -> H0 in H. simpl in H. congruence. 
- intros.
- assert (tsubst_typexpr ((tv, texp0) :: nil) texp1 = texp1).
- apply IHtexp1.
- trivial.
- assert (tsubst_typexpr ((tv, texp0) :: nil) texp2 = texp2).
- apply IHtexp2.
- trivial.
- simpl.
- rewrite -> H2.
- rewrite -> H3.
- reflexivity.
- simpl in H.
- case_eq (occurs tv texp1).
- intros.
- rewrite -> H0 in H.
- simpl in H.
- congruence.
- intros. case_eq (occurs tv texp2). intros. 
- rewrite -> H1 in H. rewrite -> H0 in H. simpl in H. congruence. 
- intros.
- assert (tsubst_typexpr ((tv, texp0) :: nil) texp1 = texp1).
- apply IHtexp1.
- trivial.
- assert (tsubst_typexpr ((tv, texp0) :: nil) texp2 = texp2).
- apply IHtexp2.
- trivial.
- simpl.
- rewrite -> H2.
- rewrite -> H3.
- reflexivity.
- simpl in H.
- assert (tsubst_typexpr ((tv, texp0) :: nil) texp = texp).
- apply IHtexp.
- trivial.
- simpl.
- rewrite -> H0.
- reflexivity.
- simpl in H.
- case_eq (occurs tv texp1).
- intros.
- rewrite -> H0 in H.
- simpl in H.
- congruence.
- intros. case_eq (occurs tv texp2). intros. 
- rewrite -> H1 in H. rewrite -> H0 in H. simpl in H. congruence. 
- intros.
- assert (tsubst_typexpr ((tv, texp0) :: nil) texp1 = texp1).
- apply IHtexp1.
- trivial.
- assert (tsubst_typexpr ((tv, texp0) :: nil) texp2 = texp2).
- apply IHtexp2.
- trivial.
- simpl.
- rewrite -> H2.
- rewrite -> H3.
- reflexivity.
-Qed.
-
-
-Theorem mgu_unifies : forall (e1 e2 : typexpr) (l : list (typvar*typexpr)), (mgu e1 e2 = Some l -> ((tsubst_typexpr l e1)=(tsubst_typexpr l e2))).
-Proof.
- intro e1.
- intro e2.
- induction e1; induction e2.
-(* var - var *)
- intros.
- simpl in H.
- destruct (eq_typvar typvar5 typvar0).
- cut ((typvar5, TE_var typvar0) :: nil = l).
- intros.
- rewrite <- H0.
- simpl.
- destruct (eq_typvar typvar5 typvar5).
- destruct (eq_typvar typvar5 typvar0).
- reflexivity.
- reflexivity.
- assert (typvar5 = typvar5).
- reflexivity.
- contradiction.
- simpl in H.
- congruence.
- assert  ((typvar5, TE_var typvar0) :: nil = l).
- congruence.
- rewrite <- H0.
- simpl.
- destruct (eq_typvar typvar5 typvar5).
- destruct (eq_typvar typvar5 typvar0).
- reflexivity.
- reflexivity.
- destruct (eq_typvar typvar5 typvar0).
- contradiction.
- assert (typvar5 = typvar5).
- reflexivity.
- contradiction.
-(* var - arrow*)
- intros.
- simpl in H.
- case_eq (occurs typvar5 e2_1).
- intros.
- rewrite -> H0 in H.
- simpl in H.
- congruence.
- intros.
- rewrite -> H0 in H.
- simpl in H.
- case_eq (occurs typvar5 e2_2).
- intros.
- rewrite -> H1 in H.
- simpl in H.
- congruence.
- intros.
- rewrite -> H1 in H.
- simpl in H.
- assert (((typvar5, TE_arrow e2_1 e2_2) :: nil) = l).
- congruence.
- auto.
- assert ((occurs typvar5 (TE_arrow e2_1 e2_2)) = false).
- simpl.
- rewrite -> H0.
- rewrite -> H1.
- auto.
- rewrite <- H2.
- assert ((tsubst_typexpr ((typvar5, TE_arrow e2_1 e2_2) :: nil) (TE_arrow e2_1 e2_2)) = (TE_arrow e2_1 e2_2)).
- apply empty_sub.
- trivial.
- rewrite -> H4.
- simpl.
- destruct (eq_typvar typvar5 typvar5).
- reflexivity.
- congruence.
-(* var - prod *)
- intros. 
- simpl in H.
- case_eq (occurs typvar5 e2_1).
- intros.
- rewrite -> H0 in H.
- simpl in H.
- congruence.
- intros.
- rewrite -> H0 in H.
- simpl in H.
- case_eq (occurs typvar5 e2_2).
- intros.
- rewrite -> H1 in H.
- simpl in H.
- congruence.
- intros.
- rewrite -> H1 in H.
- simpl in H.
- assert (((typvar5, TE_prod e2_1 e2_2) :: nil) = l).
- congruence.
- auto.
- assert ((occurs typvar5 (TE_prod e2_1 e2_2)) = false).
- simpl.
- rewrite -> H0.
- rewrite -> H1.
- auto.
- rewrite <- H2.
- assert ((tsubst_typexpr ((typvar5, TE_prod e2_1 e2_2) :: nil) (TE_prod e2_1 e2_2)) = (TE_prod e2_1 e2_2)).
- apply empty_sub.
- trivial.
- rewrite -> H4.
- simpl.
- destruct (eq_typvar typvar5 typvar5).
- reflexivity.
- congruence.
-(* var - concurrent *)
- intros.
- simpl in H.
- case_eq (occurs typvar5 e2).
- intros.
- rewrite -> H0 in H.
- congruence.
- intros.
- rewrite -> H0 in H.
- assert (((typvar5, TE_concurrent e2) :: nil) = l).
- congruence.
- rewrite <- H1.
- assert ((tsubst_typexpr ((typvar5, TE_concurrent e2) :: nil) (TE_concurrent e2)) = (TE_concurrent e2)).
- apply empty_sub.
- simpl.
- trivial.
- rewrite -> H2.
- simpl.
- destruct (eq_typvar typvar5 typvar5).
- reflexivity.
- congruence.
-(* var - sum *)
- intros.
- simpl in H.
- case_eq (occurs typvar5 e2_1).
- intros.
- rewrite -> H0 in H.
- simpl in H.
- congruence.
- intros.
- rewrite -> H0 in H.
- simpl in H.
- case_eq (occurs typvar5 e2_2).
- intros.
- rewrite -> H1 in H.
- simpl in H.
- congruence.
- intros.
- rewrite -> H1 in H.
- simpl in H.
- assert (((typvar5, TE_sum e2_1 e2_2) :: nil) = l).
- congruence.
- auto.
- assert ((occurs typvar5 (TE_sum e2_1 e2_2)) = false).
- simpl.
- rewrite -> H0.
- rewrite -> H1.
- auto.
- rewrite <- H2.
- assert ((tsubst_typexpr ((typvar5, TE_sum e2_1 e2_2) :: nil) (TE_sum e2_1 e2_2)) = (TE_sum e2_1 e2_2)).
- apply empty_sub.
- trivial.
- rewrite -> H4.
- simpl.
- destruct (eq_typvar typvar5 typvar5).
- reflexivity.
- congruence.
-(* arrow *)
- simpl.
- intro l0.
- intros.
- simpl in H.
-(* arrow - var *)
- simpl in H.
- case_eq (occurs typvar5 e1_1).
- intros.
- rewrite -> H0 in H.
- simpl in H.
- congruence.
- intros.
- rewrite -> H0 in H.
- case_eq (occurs typvar5 e1_2).
- intros.
- rewrite -> H1 in H.
- simpl in H.
- congruence.
- intros.
- rewrite -> H1 in H.
- simpl in H.
- assert (((typvar5, TE_arrow e1_1 e1_2) :: nil) = l0).
- congruence.
- rewrite <- H2.
- assert ((tsubst_typexpr ((typvar5, TE_arrow e1_1 e1_2) :: nil) e1_1) = (e1_1)).
- apply empty_sub.
- trivial.
- assert ((tsubst_typexpr ((typvar5, TE_arrow e1_1 e1_2) :: nil) e1_2) = (e1_2)).
- apply empty_sub.
- trivial.
- rewrite -> H3.
- rewrite -> H4.
- simpl.
- destruct (eq_typvar typvar5 typvar5).
- reflexivity.
- congruence.
-(* arrow - arrow *)
- intro l0.
- intros.
- simpl in H.
- case_eq (mgu e1_1 e2_1).
- intro l.
- intro.
- rewrite -> H0 in H.
- simpl H.
- case_eq (mgu (tsubst_typexpr l e1_2) e2_2).
- intro l'.
- intros.
- rewrite -> H1 in H.
- assert ((l ++ l') = l0).
- congruence.
- simpl.
- constructor 2.
- simpl.
-(* assert (tsubst_typexpr l e1_1 = tsubst_typexpr l (TE_arrow e2_1 e2_2)).
- apply IHe1_1.
- simpl in H. *)
-Admitted.
-
-
-
-
-Inductive constraint : Set := 
- | constr (s : typexpr) (t : typexpr).
-
-Fixpoint TypeCheckConstr (G5 : G) (e : expr) (T: typexpr) (X : list_typvar) (constrs : list constraint) : bool :=
-  match e with 
-  | (E_ident x) => false
-  | (E_function (value_name5:value_name) (typexpr5:typexpr) (expr5:expr)) => 
-       match T with
-       | TE_arrow (typexpr6:typexpr) (typexpr7:typexpr) => if (eq_typexpr typexpr5 typexpr6) 
-                                                           then TypeCheckConstr (G_vn G5 (value_name5) (generalise G5 typexpr5)) expr5 typexpr7 X constrs 
-                                                           else false                                                                 
-       | _ => false
-       end
-  | E_apply (e1:expr) (e2:expr) =>  
-
-
-Fixpoint InferType (G5 : G) (e : expr) : option typscheme :=
- let infT (G5 : G) (e : expr) (usedTV : list_typvar) : option typscheme :=
- match e with 
- | (E_ident x) => match GetTS x G5 with 
-                   | Some ts => Some ts
-                   | None => let ntv := newTV usedTV in Some (TS_ts (Cons_list_typvar (ntv) Nil_list_typvar) (TE_var (ntv)))
-                  end
- | (E_apply e' e'') => let ts1 := InferType G5 e' in
-                       let ts2 := InferType G5 e'' in 
-                        match ts1 with 
-                        | Some (TS_ts tvs texp) =>
-                           match texp with 
-                           | TE_arrow texparg texpret => None
-                           | _ => None
-                           end
-                        | _ => None
-                        end
-  | _ => None                                     
-end
-in infT (G5 : G) (e : expr) Nil_list_typvar.
-
-Fixpoint Typecheck (G5 : G) (e : expr) (t : typexpr) : bool :=
- match e with 
-  | E_constant CONST_ret => match t with | (TE_arrow t' (TE_concurrent t'')) =>  if eq_typexpr t' t'' then true else false | _ => false end
-  | E_constant CONST_fork => match t with 
-                             | (TE_arrow  (TE_concurrent t1)   (TE_arrow  (TE_concurrent t2)   (TE_concurrent  (TE_sum  (TE_sum  (TE_prod t1' t2')   (TE_prod t1''  (TE_concurrent t2'') ) )   (TE_prod  (TE_concurrent t1''')  t2''') ) ) ) )
-                               => if eq_typexpr t1 t1' then if eq_typexpr t1' t1'' then if eq_typexpr t1'' t1''' then if eq_typexpr t2 t2' then if eq_typexpr t2' t2'' then if eq_typexpr t2'' t2''' then true else false else false else false else false else false else false
-                             | _ => false
-                             end
-  | E_apply e' e'' => match t with | TE_arrow t' t'' => andb (Typecheck G5 e' t') (Typecheck G5 e'' t'') | _ => false end
-  | E_function x1 t1 e1 => match t with | (TE_arrow t1 t2) => Typecheck (G_vn G5 x1 (TS_ts Nil_list_typvar t1)) e1 t2 | _ => false end
-  | E_live_expr e1 => match t with | (TE_concurrent t1) => Typecheck G5 e1 t1 | _ => false end
-  | E_bind e1 e2 => false
-  | _ => false
- end. 
-*)
+Recursive Extraction selectstar.
 
 (* Extractable version of the reduction operation *)
-Inductive XJO_red : expr -> expr -> Prop :=    (* defn red *)
- | XJO_red_app : forall (x:value_name) (t : typexpr) (e v:expr),
+Inductive XJO_red : expr -> selectstar -> expr -> Prop :=    (* defn red *)
+ | XJO_red_app : forall (x:value_name) (t : typexpr) (e v:expr) (s:selectstar),
      (eq (xis_value_of_expr v) true) ->
-     XJO_red (E_apply  (E_function x t e)  v)  (subst_expr  v   x   e ) 
- | XJO_red_forkmove1 : forall (e e' e'':expr),
-     (eq select First) ->  
-     (eq (xis_value_of_expr e) false) ->
-     (eq (xis_value_of_expr e') false) ->   
-     XJO_red e e'' ->
-     XJO_red (E_apply  (E_apply (E_constant CONST_fork)  (E_live_expr e) )   (E_live_expr e') ) (E_apply  (E_apply (E_constant CONST_fork)  (E_live_expr e'') )   (E_live_expr e') )
- | XJO_red_forkmove2 : forall (e e' e'':expr),
-     (eq select Second) ->
+     XJO_red (E_apply  (E_function x t e)  v) s  (subst_expr  v   x   e ) 
+ | XJO_red_ret : forall (v:expr) (s:selectstar),
+     (eq (xis_value_of_expr v) true) ->
+     XJO_red (E_apply (E_constant CONST_ret) v) s (E_live_expr (LM_expr (v))) 
+ | XJO_red_evalbind : forall (e e'' e':expr) (s:selectstar),
+     XJO_red e s e' ->
+     XJO_red (E_bind e e'') s (E_bind e' e'')
+ | XJO_red_movebind : forall (e e'' e':expr) (s:selectstar),
      (eq (xis_value_of_expr e) false) -> 
-     (eq (xis_value_of_expr e') false) -> 
-     XJO_red e' e'' ->
-     XJO_red (E_apply  (E_apply (E_constant CONST_fork)  (E_live_expr e) )   (E_live_expr e') ) (E_apply  (E_apply (E_constant CONST_fork)  (E_live_expr e) )   (E_live_expr e'') )
-(* | XJO_red_forkmove12 : forall (e e' e'' e''':expr),
-     (eq select Both) ->
-     (eq (xis_value_of_expr e) false) ->
-     (eq (xis_value_of_expr e') false) ->
-     XJO_red e e'' ->
-     XJO_red e' e''' ->
-     XJO_red (E_apply  (E_apply (E_constant CONST_fork)  (E_live_expr e) )   (E_live_expr e') ) (E_apply  (E_apply (E_constant CONST_fork)  (E_live_expr e'') )   (E_live_expr e''') )
-*) | XJO_red_forkdeath1 : forall (v e':expr),
+     XJO_red e s e' ->
+     XJO_red (E_bind  (E_live_expr (LM_expr (e)))  e'') s (E_bind  (E_live_expr (LM_expr (e')))  e'')
+ | XJO_red_dobind : forall (v e:expr) (s:selectstar),
      (eq (xis_value_of_expr v) true) ->
+     XJO_red (E_bind  (E_live_expr (LM_expr (v)))  e) s (E_apply e v) 
+ | XJO_red_context_app1 : forall (e e' e'':expr) (s:selectstar),
      (eq (xis_value_of_expr e') false) ->
-     XJO_red (E_apply  (E_apply (E_constant CONST_fork)  (E_live_expr v) )   (E_live_expr e') ) (E_live_expr (E_pair v  (E_live_expr e') ))
- | XJO_red_forkdeath2 : forall (v e:expr),
+     XJO_red e' s e'' ->
+     XJO_red (E_apply e e') s (E_apply e e'')
+ | XJO_red_context_app2 : forall (e v e':expr) (s:selectstar),
      (eq (xis_value_of_expr v) true) ->
-     (eq (xis_value_of_expr e) false) ->
-     XJO_red (E_apply  (E_apply (E_constant CONST_fork)  (E_live_expr e) )   (E_live_expr v) ) (E_live_expr (E_pair  (E_live_expr e)  v))
- | XJO_red_forkdeath12 : forall (v v':expr),
+     XJO_red e s e' ->
+     XJO_red (E_apply e v) s (E_apply e' v)
+ | XJO_red_forkeval2 : forall (v v' e':expr) (s :selectstar),
+     (eq (xis_value_of_expr v') false) ->
+     XJO_red v' s e' ->
+     XJO_red (E_apply  (E_apply (E_constant CONST_fork) v )  v') s (E_apply  (E_apply (E_constant CONST_fork) v )  e')
+ | XJO_red_forkeval1 : forall (v e':expr) (lm : livemodes) (s:selectstar),
+     (eq (xis_value_of_expr v) false) ->
+     XJO_red v s e' ->
+     XJO_red (E_apply  (E_apply (E_constant CONST_fork) v )  (E_live_expr lm)) s (E_apply  (E_apply (E_constant CONST_fork) e' )  (E_live_expr lm))
+ | XJO_red_forkdeath12 : forall (v v':expr) (s:selectstar),
      (eq (xis_value_of_expr v) true) ->
      (eq (xis_value_of_expr v') true)->
-     XJO_red (E_apply  (E_apply (E_constant CONST_fork)  (E_live_expr v) )   (E_live_expr v') ) (E_live_expr (E_pair v v'))
- | XJO_red_ret : forall (v:expr),
-     (eq (xis_value_of_expr v) true) ->
-     XJO_red (E_apply (E_constant CONST_ret) v) (E_live_expr v)
- | XJO_red_evalbind : forall (e e'' e':expr),
-     XJO_red e e' ->
-     XJO_red (E_bind e e'') (E_bind e' e'')
- | XJO_red_movebind : forall (e e'' e':expr),
-     (eq (xis_value_of_expr e) false) -> 
-     XJO_red e e' ->
-     XJO_red (E_bind  (E_live_expr e)  e'') (E_bind  (E_live_expr e')  e'')
- | XJO_red_dobind : forall (v e:expr),
-     (eq (xis_value_of_expr v) true) ->
-     XJO_red (E_bind  (E_live_expr v)  e) (E_apply e v)
- | XJO_red_context_app1 : forall (e e' e'':expr),
+     XJO_red (E_apply  (E_apply (E_constant CONST_fork)  (E_live_expr (LM_expr (v))) )   (E_live_expr (LM_expr (v'))) ) s (E_live_expr (LM_expr(E_pair v v')))
+ | XJO_red_forkdeath1 : forall (e e':expr) (s:selectstar),
+     (eq (xis_value_of_expr e) true) ->
      (eq (xis_value_of_expr e') false) ->
-     XJO_red e' e'' ->
-     XJO_red (E_apply e e') (E_apply e e'')
- | XJO_red_context_app2 : forall (e v e':expr),
-     (eq (xis_value_of_expr v) true) ->
-     XJO_red e e' ->
-     XJO_red (E_apply e v) (E_apply e' v)
- | XJO_red_pair_1 : forall (e e'' e':expr),
+     XJO_red (E_apply  (E_apply (E_constant CONST_fork)  (E_live_expr (LM_expr (e))) )   (E_live_expr (LM_expr (e'))) ) s (E_live_expr (LM_expr(E_pair e  (E_live_expr (LM_expr (e')))) ))
+ | XJO_red_forkdeath2 : forall (e e':expr) (s:selectstar),
      (eq (xis_value_of_expr e) false) ->
-     XJO_red e e' ->
-     XJO_red (E_pair e e'') (E_pair e' e'')
- | XJO_red_pair_2 : forall (v e e':expr),
+     (eq (xis_value_of_expr e') true) ->
+     XJO_red (E_apply  (E_apply (E_constant CONST_fork)  (E_live_expr (LM_expr (e))) )   (E_live_expr (LM_expr (e'))) ) s (E_live_expr (LM_expr(E_pair  (E_live_expr (LM_expr (e)))  e')))
+ | XJO_red_forkmove1 : forall (v v' e'':expr) (s:selectstar),  
+     (eq (xis_value_of_expr v) false) ->
+     (eq (xis_value_of_expr v') false) ->   
+     XJO_red v s e'' ->
+     XJO_red (E_apply  (E_apply (E_constant CONST_fork)  (E_live_expr (LM_expr (v))) )   (E_live_expr (LM_expr (v'))) ) (Seq S_First s) (E_apply  (E_apply (E_constant CONST_fork)  (E_live_expr (LM_expr (e''))) )   (E_live_expr (LM_expr (v'))) )
+ | XJO_red_forkmove2 : forall (e e' e'':expr) (s:selectstar),
+     (eq (xis_value_of_expr e) false) -> 
+     (eq (xis_value_of_expr e') false) -> 
+     XJO_red e' s e'' ->
+     XJO_red (E_apply  (E_apply (E_constant CONST_fork)  (E_live_expr (LM_expr (e))) )   (E_live_expr (LM_expr (e'))) ) (Seq S_Second s) (E_apply  (E_apply (E_constant CONST_fork)  (E_live_expr (LM_expr (e))) )   (E_live_expr (LM_expr (e''))) )
+(*| XJO_red_forkdocomp1 : forall (e:expr) (s:selectstar),
+     XJO_red (E_apply  (E_apply (E_constant CONST_fork)  (E_live_expr LM_comp) )   (E_live_expr (LM_expr e)) ) s (E_live_expr (LM_expr  (E_taggingleft  (E_taggingright  (E_pair (E_constant CONST_unit)  (E_live_expr (LM_expr e)) ) ) ) ))
+ | XJO_red_forkdocomp2 : forall (e:expr) (s:selectstar),
+     XJO_red (E_apply  (E_apply (E_constant CONST_fork)  (E_live_expr (LM_expr e)) )   (E_live_expr LM_comp) ) s (E_live_expr (LM_expr  (E_taggingright  (E_pair  (E_live_expr (LM_expr e))  (E_constant CONST_unit)) ) ))
+ | XJO_red_forkdocomp12 : forall (s:selectstar),
+     XJO_red (E_apply  (E_apply (E_constant CONST_fork)  (E_live_expr LM_comp) )   (E_live_expr LM_comp) ) s (E_live_expr (LM_expr  (E_taggingleft  (E_taggingleft  (E_pair (E_constant CONST_unit) (E_constant CONST_unit)) ) ) ))
+(* | XJO_red_forkdeathfp1 : forall (v v':expr),
+     (eq (xis_value_of_expr v') true) ->
      (eq (xis_value_of_expr v) true) ->
-     XJO_red e e' ->
-     XJO_red (E_pair v e) (E_pair v e')
- | XJO_red_evalinl : forall (e e':expr),
-     XJO_red e e' ->
-     XJO_red (E_taggingleft e) (E_taggingleft e')
- | XJO_red_evalinr : forall (e e':expr),
-     XJO_red e e' ->
-     XJO_red (E_taggingright e) (E_taggingright e')
- | XJO_red_evalcaseinl : forall (x:value_name) (e:expr) (x':value_name) (e' v:expr),
+     (eq (xis_forkvalue v) true) ->
+     (eq (xis_forkvalue v') false) ->
+     XJO_red (E_apply  (E_apply (E_constant CONST_fork) v )  v') (E_live_expr (E_pair v v'))
+ | XJO_red_forkdeathfp2 : forall (v v':expr),
+     (eq (xis_value_of_expr v') true) ->
      (eq (xis_value_of_expr v) true) ->
-     XJO_red (E_case  (E_taggingleft v)  x e x' e')  (subst_expr  v   x   e ) 
- | XJO_red_evalcaseinr : forall (x:value_name) (e:expr) (x':value_name) (e' v:expr),
+     (eq (xis_forkvalue v) false) ->
+     (eq (xis_forkvalue v') true) ->
+     XJO_red (E_apply  (E_apply (E_constant CONST_fork) v )  v') (E_live_expr (E_pair v v'))
+ | XJO_red_forkdeathfp12 : forall (v v':expr),
+     (eq (xis_value_of_expr v') true) ->
      (eq (xis_value_of_expr v) true) ->
-     XJO_red (E_case  (E_taggingright v)  x e x' e')  (subst_expr  v   x'   e' ) 
- | XJO_red_evalcase : forall (e:expr) (x:value_name) (e'':expr) (x':value_name) (e''' e':expr),
+     (eq (xis_forkvalue v) true) ->
+     (eq (xis_forkvalue v') true) ->
+     XJO_red (E_apply  (E_apply (E_constant CONST_fork) v )  v') (E_live_expr (E_pair v v')) *)
+(* | XJO_red_forkdeathfp2 : forall (v v':expr)
+     (eq (xis_value_of_expr v) true) ->
+     (eq (xis_value_of_expr v') true) ->
+     XJO_red (E_apply  (E_apply (E_constant CONST_fork) v)   (E_apply (E_constant CONST_fork) v') ) (E_live_expr (E_pair v  (E_apply (E_constant CONST_fork) v') ))
+ | XJO_red_forkdeathret1 : forall (v:expr),
+     (eq (xis_value_of_expr v) true) ->
+     XJO_red (E_apply  (E_apply (E_constant CONST_fork) (E_constant CONST_ret))  v) (E_live_expr (E_pair (E_constant CONST_ret) v))
+ | XJO_red_forkdeathret2 : forall (v:expr),
+     (eq (xis_value_of_expr v) true) ->
+     XJO_red (E_apply  (E_apply (E_constant CONST_fork) v)  (E_constant CONST_ret)) (E_live_expr (E_pair v (E_constant CONST_ret)))
+*)
+ | XJO_red_pair_1 : forall (e e'' e':expr) (s:selectstar),
      (eq (xis_value_of_expr e) false) ->
-     XJO_red e e' ->
-     XJO_red (E_case e x e'' x' e''') (E_case e' x e'' x' e''').  
+     XJO_red e s e' ->
+     XJO_red (E_pair e e'') s (E_pair e' e'')
+ | XJO_red_pair_2 : forall (v e e':expr)(s s':selectstar),
+     (eq (xis_value_of_expr v) true) ->
+     XJO_red e s e' ->
+     XJO_red (E_pair v e) s' (E_pair v e')
+ | XJO_red_evalinl : forall (e e':expr)(s:selectstar),
+     XJO_red e s e' ->
+     XJO_red (E_taggingleft e) s (E_taggingleft e')
+ | XJO_red_evalinr : forall (e e':expr) (s:selectstar),
+     XJO_red e s e' ->
+     XJO_red (E_taggingright e) s (E_taggingright e')
+ | XJO_red_evalcaseinl : forall (x:value_name) (e:expr) (x':value_name) (e' v:expr)(s:selectstar),
+     (eq (xis_value_of_expr v) true) ->
+     XJO_red (E_case  (E_taggingleft v)  x e x' e') s  (subst_expr  v   x   e ) 
+ | XJO_red_evalcaseinr : forall (x:value_name) (e:expr) (x':value_name) (e' v:expr)(s:selectstar),
+     (eq (xis_value_of_expr v) true) ->
+     XJO_red (E_case  (E_taggingright v)  x e x' e') s  (subst_expr  v   x'   e' ) 
+ | XJO_red_evalcase : forall (e:expr) (x:value_name) (e'':expr) (x':value_name) (e''' e':expr) (s:selectstar),
+     (eq (xis_value_of_expr e) false) ->
+     XJO_red e s e' ->
+     XJO_red (E_case e x e'' x' e''') s (E_case e' x e'' x' e''') *).  
 
-(* Proof that if a term reduces, it is not a value *)
-
-Lemma red_not_value : forall (e : expr) (e' : expr), (JO_red e e') -> (~(is_value_of_expr e)).
-Proof.
- intro e.
- induction e.
- intros.
- inversion H.
- intros.
- inversion H.
- simpl.
- trivial.
- simpl.
- trivial.
- intros.
- induction e1. 
- auto.
- case_eq constant5.
- intros; auto.
- intros.
- rewrite -> H0 in H.
- inversion H.
- apply IHe2 with (e' := e'').
- trivial.
- inversion H5.
- auto.
- auto. 
- auto.
- auto. 
- auto. 
- auto.
- auto.
- auto.
- intros.
- simpl.
- auto.
- intros.
- inversion H.
- intros.
- simpl; auto.
- inversion H.
- intros.
- simpl.
- unfold not.
- intros.
- elim H0.
- intros.
- inversion H.
- assert  (~ is_value_of_expr e1).
- apply IHe1 with (e' := e'0).
- trivial.
- contradiction.
- assert  (~ is_value_of_expr e2).
- apply IHe2 with (e' := e'0).
- trivial.
- contradiction.
- assert (is_value_of_expr e1).
- rewrite <- H0.
- simpl.
- auto.
- contradiction.
- apply IHe1 in H7.
- rewrite <- H0 in H7.
- unfold not in H7.
- apply H7.
- simpl.
- auto.
- apply IHe1 in H7.
- rewrite <- H0 in H7.
- unfold not in H7.
- apply H7.
- simpl.
- auto.
- simpl.
- auto.
- simpl; auto.
- simpl; auto.
- intros.
- simpl.
- inversion H.
- intros.
- inversion H.
- intros.
- inversion H.
- apply IHe1 in H3.
- simpl.
- unfold not.
- intros. 
- elim H4.
- intros; contradiction.
- simpl.
- unfold not; intros.
- elim H5.
- intros.
- apply IHe2 in H4.
- contradiction.
- intros.
- inversion H.
- apply IHe in H1.
- simpl.
- trivial.
- intros.
- inversion H.
- simpl.
- apply IHe in H1.
- trivial.
- intros.
- simpl.
- auto.
-Qed.
-
-Lemma empty_VTSin_false : forall  (v : value_name)  (ts : typscheme), ~ (VTSin v ts G_em).
-Proof.
- intros.
- unfold not.
- intros.
- inversion H.
-Qed.
-
-Lemma is_value_of_expr_dec : forall (e : expr), ((is_value_of_expr e) \/ (~(is_value_of_expr e))).
- Proof.
- intros.
- apply classic.
-Qed.
-
- 
-(*
-Lemma not_value_red : forall (e : expr), (~(is_value_of_expr e) /\ (exists (t : typexpr), Get G_em e t)) -> (exists (e' : expr), (JO_red e e')).
-Proof.
- intro e.
- induction e.
- intros.
- simpl in H.
- elim H.
- intros.
- elim H1.
- intros.
- inversion H2.
- assert (~ (VTSin value_name5 typscheme5 G_em)).
- apply empty_VTSin_false.
- contradiction.
- intros.
- elim H.
- intros.
- assert (is_value_of_expr (E_constant constant5)).
- simpl.
- trivial.
- contradiction.
- intros.
- elim H.
- intros.
- elim H1.
- intros.
- inversion H2.
- assert ((is_value_of_expr e2) \/ (~(is_value_of_expr e2))).
- apply is_value_of_expr_dec.
- elim H9.
- intros.
- inversion H6.
- assert (~(VTSin x0 typscheme5 G_em)).
- apply empty_VTSin_false.
- contradiction.
- inversion H11.
- exists ((E_live_expr e2)).
- apply JO_red_ret.
- trivial.
- rewrite <- H13 in H0.
- rewrite <- H16 in H0.
- simpl in H0.
- contradiction.
- inversion H11.
- apply empty_VTSin_false in H16.
- elim H16.
- inversion H16.
- rewrite <- H23 in H12. 
- rewrite <- H24 in H8.
- assert ((exists e2' : expr, JO_red e2 e2') \/ ~ (exists e2' : expr, JO_red e2 e2')).
- apply classic with (P :=  (exists e2' : expr, JO_red e2 e2')).
- elim H22.
- intros.
- elim H26.
- intros.
- assert (JO_red (E_apply (E_apply (E_constant CONST_fork) e'0) e2) (E_apply (E_apply (E_constant CONST_fork) e'0) x0)).
- apply JO_red_context_app1.
- trivial.
- exists ((E_apply (E_apply (E_constant CONST_fork) e'0) x0)).
- trivial.
- intros.
- assert ((exists y : expr, JO_red e'0 y) \/ ~ (exists y : expr, JO_red e'0 y)).
- apply classic with (P :=  (exists y : expr, JO_red e'0 y)).
- elim H27.
- intros.
- elim H28.
- intros.
- assert (JO_red  (E_apply (E_constant CONST_fork) e'0) (E_apply (E_constant CONST_fork) x0)).
- apply JO_red_context_app1.
- trivial.
- assert (JO_red (E_apply (E_apply (E_constant CONST_fork) e'0) e2) (E_apply (E_apply (E_constant CONST_fork) x0) e2)).
- apply JO_red_context_app2.
- assert ((is_value_of_expr e2) \/ ~(is_value_of_expr e2)).
- apply classic.
- elim H31.
- intros; trivial.
- intros.
- assert (exists e' : expr, JO_red e2 e').
- apply IHe2.
- split.
- trivial.
- exists ((TE_concurrent t5)).
- trivial.
- unfold not in H26.
- auto.
- trivial.
- exists ((E_apply (E_apply (E_constant CONST_fork) x0) e2)).
- trivial.
- intros.
- assert ((is_value_of_expr e2) \/ ~(is_value_of_expr e2)).
- apply classic.
- elim H29.
- intros.
- induction e2.
- simpl in H30.
- elim H30.
- induction constant0.
- inversion H8.
- inversion H33.
- inversion H8.
- inversion H33. 
- simpl in H30.
- 
- induction e2_1.
- simpl in H30; elim H30.
- simpl in H30.
- induction constant0.
- simpl in H30; elim H30.
- 
-
- rewrite <- H14 in H2.
- simpl in H2.
-
- exists ((E_apply (E_apply (E_constant CONST_fork) e'0) x0)).
- trivial.
- intros. 
-
-
- auto.
-
- inversion H8.
- apply empty_VTSin_false in H22.
- elim H22.
- assert 
- inversion H22.
- simpl in H22.
- 
- case (is_value_of_expr e2).
- simpl.
- simpl H2. 
-
- auto.
- simpl.
- simpl. 
-
-
- inversion H4.
- intros.
- elim H.
- intros.
- simpl in H0.
- assert False.
- unfold not in H0.
- apply H0.
- trivial.
- absurd (False).
- unfold not.
- intros. 
- trivial.
- trivial.
- intros.
- elim H.
- intros.
- elim H1.
- intros.
- inversion H2.
- inversion H6.
- rewrite <- H12 in H6.
- inversion H6.
- inversion JO_red.
- simpl.
- simpl H2.
- case_eq H4.
- intros.
- inversion in H4.
- simpl in H4.
- simpl in H.
- simpl.
- 
-*)
-(* Proof that reduction and the extractable reduction is equivalent *)
- (*Theorem xred_if_red : forall (e e' : expr), JO_red e e' -> (exists (s : selectSet), (XJO_red e e')).
-Proof.
- intros.
- inversion H.
- exists First.
- apply XJO_red_app.
- apply l_val.
- trivial.
- exists First.
- apply XJO_red_forkmove1.
- apply red_not_value in H.
- apply not_true_is_false.
- apply red_not_value in H0.
- rewrite <- l_val in H0.
- trivial.
- apply First.
- apply First.
- apply red_not_value in H0.
- rewrite <- l_val in H0.
- apply not_true_is_false.
- trivial.
- trivial.
-Admitted.*) 
-(*
-Theorem red_if_xred : forall (e e' : expr), XJO_red e e' -> (JO_red e e').
-Proof.
- intro e.
- induction e.
- intros.
- inversion H.
- intros.
- inversion H.
- intros.
- inversion H.
- apply JO_red_app.
- apply l_val in H3. 
- trivial.
- apply JO_red_forkmove1.
- induction e1.
- congruence.
- congruence.
- simpl in H0.
- induction e1_2.
- congruence.
- congruence.
- congruence.
- congruence.
- congruence.
- assert (e1_1 = (E_constant CONST_fork)).
- congruence.
- assert (e = e1_2).
- congruence.
- rewrite <- H8 in H.
- rewrite <- H8 in IHe1_2.
- rewrite <- H8 in IHe1_0.
- rewrite -> H7 in H.
- rewrite -> H7 in IHe1_1.
- rewrite -> H7 in IHe1_0.
- apply IHe1_0.
- rewrite <- H8 in IHe1.
- rewrite -> H7 in IHe1.
- trivial.
- congruence.
- intros.
- inversion H.
- apply JO_red_app.
- apply l_val in H0.
- trivial.
- induction e.
- apply JO_red_forkmove1.
- simpl.
-Admitted.
-*)
 
 (*Extraction Relation Fixpoint is_expr_of_expr [1]. *)
 
 Recursive Extraction xis_value_of_expr.
 
-Extraction Relation Relaxed XJO_red [1].
+Recursive Extraction select.
 
-Recursive Extraction XVTSin.
+Recursive Extraction expr.
+
+Extraction Relation Relaxed XJO_red [1 2].
+
 
 (* Extraction Relation G_constant [1 2]. *)
